<?xml version="1.0"?>


<!DOCTYPE rdf:RDF [
    <!ENTITY owl "http://www.w3.org/2002/07/owl#" >
    <!ENTITY xsd "http://www.w3.org/2001/XMLSchema#" >
    <!ENTITY xml "http://www.w3.org/XML/1998/namespace" >
    <!ENTITY rdfs "http://www.w3.org/2000/01/rdf-schema#" >
    <!ENTITY rdf "http://www.w3.org/1999/02/22-rdf-syntax-ns#" >
]>


<rdf:RDF xmlns="http://purl.org/net/wfd#"
     xml:base="http://purl.org/net/wfd"
     xmlns:rdfs="http://www.w3.org/2000/01/rdf-schema#"
	 xmlns:terms="http://purl.org/dc/terms/"
	 xmlns:vann="http://purl.org/vocab/vann/"
	 xmlns:prov="http://www.w3.org/ns/prov#"
     xmlns:owl="http://www.w3.org/2002/07/owl#"
     xmlns:xsd="http://www.w3.org/2001/XMLSchema#"
     xmlns:rdf="http://www.w3.org/1999/02/22-rdf-syntax-ns#"
     xmlns:xml="http://www.w3.org/XML/1998/namespace">
    <owl:Ontology rdf:about="http://purl.org/net/wf-fd#">
        <rdfs:label xml:lang="en">Workflow Fragment Description Ontology</rdfs:label>
		<terms:created rdf:datatype="&xsd;date">2012-07-17</terms:created>
        <terms:modified rdf:datatype="&xsd;date">2013-07-17</terms:modified>
        <terms:creator rdf:datatype="&xsd;anyURI">http://delicias.dia.fi.upm.es/members/DGarijo/#me</terms:creator>        
        <vann:preferredNamespacePrefix>wffd</vann:preferredNamespacePrefix>
        <terms:license>http://creativecommons.org/licenses/by-nc-sa/2.0/</terms:license>
        <vann:preferredNamespaceUri>http://purl.org/net/wf-fd#</vann:preferredNamespaceUri>
        <owl:versionInfo>1.0</owl:versionInfo>
        <terms:description xml:lang="en">P-Plan extension to represent workflow fragments and their relationships to workflow templates</terms:description>
        <rdfs:comment>P-Plan extension to represent workflow fragments and their relationships to workflow templates</rdfs:comment>
        <terms:title xml:lang="en">The Workflow Fragment Description ontology</terms:title>
    </owl:Ontology>
    


    <!-- 
    ///////////////////////////////////////////////////////////////////////////////////////
    //
    // Annotation properties
    //
    ///////////////////////////////////////////////////////////////////////////////////////
     -->

    


    <!-- 
    ///////////////////////////////////////////////////////////////////////////////////////
    //
    // Datatypes
    //
    ///////////////////////////////////////////////////////////////////////////////////////
     -->

    


    <!-- 
    ///////////////////////////////////////////////////////////////////////////////////////
    //
    // Object Properties
    //
    ///////////////////////////////////////////////////////////////////////////////////////
     -->

    


    <!-- http://purl.org/net/p-plan#isStepOfPlan -->

    <owl:ObjectProperty rdf:about="http://purl.org/net/p-plan#isStepOfPlan"/>
    


    <!-- http://purl.org/net/wf-fd#foundAs -->

    <owl:ObjectProperty rdf:about="http://purl.org/net/wf-fd#foundAs">
        <rdfs:label xml:lang="en">foundAs</rdfs:label>
        <rdfs:comment xml:lang="en">Property that links a Detected Result Workflow Fragment to a Bound Result Workflow Fragment. That is, this property links a workflow fragment found as a result of applying graph mining techniques to a collection of workflows to the correspondant fragment of the workflow itself.</rdfs:comment>
        <rdfs:range rdf:resource="http://purl.org/net/wf-fd#BoundResultWorkflowFragment"/>
        <rdfs:domain rdf:resource="http://purl.org/net/wf-fd#DetectedResutlWorkflowFragment"/>
    </owl:ObjectProperty>
    


    <!-- http://purl.org/net/wf-fd#isPreceededBy -->

    <owl:ObjectProperty rdf:about="http://purl.org/net/wf-fd#isPreceededBy">
        <rdf:type rdf:resource="&owl;TransitiveProperty"/>
        <rdfs:label xml:lang="en">isPreceededBy</rdfs:label>
        <rdfs:comment xml:lang="en">Property that asserts which DetectedResultFragmentStep preceeds the current one. This only affects the Fragment Steps which have been detected by the graph matching algorithms</rdfs:comment>
        <rdfs:range rdf:resource="http://purl.org/net/wf-fd#DetectedResultFragmentStep"/>
        <rdfs:domain rdf:resource="http://purl.org/net/wf-fd#DetectedResultFragmentStep"/>
    </owl:ObjectProperty>
    


    <!-- http://purl.org/net/wf-fd#isStepOfWorkflowFragment -->

    <owl:ObjectProperty rdf:about="http://purl.org/net/wf-fd#isStepOfWorkflowFragment">
        <rdfs:label xml:lang="en">isStepOfWorkflowFragment</rdfs:label>
        <rdfs:comment xml:lang="en">Property that links a Workflow Fragment Step with its corresponding Workflow Fragment. It extends the p-plan property isStepOfPlan.</rdfs:comment>
        <rdfs:subPropertyOf rdf:resource="http://purl.org/net/p-plan#isStepOfPlan"/>
        <rdfs:range rdf:resource="http://purl.org/net/wf-fd#WorkflowFragment"/>
        <rdfs:domain rdf:resource="http://purl.org/net/wf-fd#WorkflowFragmentStep"/>
    </owl:ObjectProperty>
    


    <!-- http://purl.org/net/wf-fd#overlapsWithWorkflowFragment -->

    <owl:ObjectProperty rdf:about="http://purl.org/net/wf-fd#overlapsWithWorkflowFragment">
        <rdfs:label xml:lang="en">overlapsWithWorkflowFragment</rdfs:label>
        <rdfs:comment xml:lang="en">Property that specifies which Detected Result Workflow Fragments overlap with each other. In this case an overlap means to be included partially as part of another fragment</rdfs:comment>
        <rdfs:range rdf:resource="http://purl.org/net/wf-fd#DetectedResutlWorkflowFragment"/>
        <rdfs:domain rdf:resource="http://purl.org/net/wf-fd#DetectedResutlWorkflowFragment"/>
    </owl:ObjectProperty>
    


    <!-- http://purl.org/net/wf-fd#overlapsWithWorkflowFragmentStep -->

    <owl:ObjectProperty rdf:about="http://purl.org/net/wf-fd#overlapsWithWorkflowFragmentStep">
        <rdfs:label xml:lang="en">overlapsWithWorkflowFragmentStep</rdfs:label>
        <rdfs:comment xml:lang="en">Property that links a detected Result Workflow Fragment Step with another step belonging to a fragment which overlaps with the current one. This property highlights which fragments overlap with other fragments (and how).</rdfs:comment>
        <rdfs:domain rdf:resource="http://purl.org/net/wf-fd#DetectedResultFragmentStep"/>
        <rdfs:range rdf:resource="http://purl.org/net/wf-fd#DetectedResultFragmentStep"/>
    </owl:ObjectProperty>
    


    <!-- 
    ///////////////////////////////////////////////////////////////////////////////////////
    //
    // Classes
    //
    ///////////////////////////////////////////////////////////////////////////////////////
     -->

    


    <!-- http://purl.org/net/p-plan#Plan -->

    <owl:Class rdf:about="http://purl.org/net/p-plan#Plan"/>
    


    <!-- http://purl.org/net/p-plan#Step -->

    <owl:Class rdf:about="http://purl.org/net/p-plan#Step"/>
    


    <!-- http://purl.org/net/wf-fd#BoundResultWorkflowFragment -->

    <owl:Class rdf:about="http://purl.org/net/wf-fd#BoundResultWorkflowFragment">
        <rdfs:label xml:lang="en">Bound Result Workflow Fragment</rdfs:label>
        <rdfs:subClassOf rdf:resource="http://purl.org/net/wf-fd#WorkflowFragment"/>
        <rdfs:comment xml:lang="en">A Bound Workflow Result Fragment is a Workflow Fragment used as an auxiliary structure to point to Workflow Steps of a collection of workflows. </rdfs:comment>
    </owl:Class>
    


    <!-- http://purl.org/net/wf-fd#DetectedResultFragmentStep -->

    <owl:Class rdf:about="http://purl.org/net/wf-fd#DetectedResultFragmentStep">
        <rdfs:label xml:lang="en">Detected Result Fragment Step</rdfs:label>
        <rdfs:subClassOf rdf:resource="http://purl.org/net/wf-fd#WorkflowFragmentStep"/>
        <rdfs:comment xml:lang="en">A Detected Result Fragment Step is a Step of a Workflow Fragment which has been detected by applying graph mining techniques among a collection of workflows.</rdfs:comment>
    </owl:Class>
    


    <!-- http://purl.org/net/wf-fd#DetectedResutlWorkflowFragment -->

    <owl:Class rdf:about="http://purl.org/net/wf-fd#DetectedResutlWorkflowFragment">
        <rdfs:label xml:lang="en">Detected Result Workflow Fragment</rdfs:label>
        <rdfs:subClassOf rdf:resource="http://purl.org/net/wf-fd#WorkflowFragment"/>
        <rdfs:comment xml:lang="en">A Detected Result Workflow Fragment is a Workflow Fragment detected automatically by using graph matching tecnhiques over a workflow collection. This fragment is a result of the algortihms and it is composed of Detected Result Steps.</rdfs:comment>
    </owl:Class>
    


    <!-- http://purl.org/net/wf-fd#WorkflowFragment -->

    <owl:Class rdf:about="http://purl.org/net/wf-fd#WorkflowFragment">
        <rdfs:label xml:lang="en">Workflow Fragment</rdfs:label>
        <rdfs:subClassOf rdf:resource="http://purl.org/net/p-plan#Plan"/>
        <rdfs:comment xml:lang="en">A Workflow Fragment is a set of connected steps which belongs as part of a scientific workflow. A Workflow Fragment is a directed acyclic graph (DAG) and may have one or more Steps.

There are two types of Workflow Fragments: The Bound Result Workflow Fragments and the Detected Result Workflow Fragments. On one hand, the Detected Result Workflow Fragments are used to describe the results of the graph matching algorithms applied to a workflow collection. On the other hand, the Bound Workflow Result Fragments are auxiliary structures to point out the Steps of a Workflow belonging to a Detected Result Workflow Fragment .</rdfs:comment>
    </owl:Class>
    


    <!-- http://purl.org/net/wf-fd#WorkflowFragmentStep -->

    <owl:Class rdf:about="http://purl.org/net/wf-fd#WorkflowFragmentStep">
        <rdfs:label xml:lang="en">Workflow Fragment Step</rdfs:label>
        <rdfs:subClassOf rdf:resource="http://purl.org/net/p-plan#Step"/>
        <rdfs:comment xml:lang="en">A Workflow Fragment Step is a step of a Workflow Fragment</rdfs:comment>
    </owl:Class>
</rdf:RDF>



<!-- Generated by the OWL API (version 3.3.1957) http://owlapi.sourceforge.net -->

